src/HarvardMachine.v
@@ -24,61 +24,15 @@ Section Riscv.
 
   Definition InstructionMem := word wXLEN -> Instruction.
   
-  Record HarvardMachine := mkHarvardMachine {
-    machine: @RiscvMachine _ (mem wXLEN);
-    instructionMem: InstructionMem;
-  }.
-
-  Definition with_machine m ml := mkHarvardMachine m ml.(instructionMem).
-  Definition with_instructionMem l ml := mkHarvardMachine ml.(machine) l.  
-
-  Definition liftL0{B: Type}(f: OState RiscvMachine B):  OState HarvardMachine B :=
-    fun s => let (ob, ma) := f s.(machine) in (ob, with_machine ma s).
-
-  Definition liftL1{A B: Type}(f: A -> OState RiscvMachine B): A -> OState HarvardMachine B :=
-    fun a s => let (ob, ma) := f a s.(machine) in (ob, with_machine ma s).
-
-  Definition liftL2{A1 A2 B: Type}(f: A1 -> A2 -> OState RiscvMachine B):
-    A1 -> A2 -> OState HarvardMachine B :=
-    fun a1 a2 s => let (ob, ma) := f a1 a2 s.(machine) in (ob, with_machine ma s).
-                                           
-  Instance IsHarvardMachine: RiscvProgram (OState HarvardMachine) (word wXLEN) :=  {|
-      getRegister := liftL1 getRegister;
-      setRegister := liftL2 setRegister;
-      getPC := liftL0 getPC;
-      setPC := liftL1 setPC;
-      loadByte   := liftL1 loadByte;
-      loadHalf   := liftL1 loadHalf;
-      loadWord   := liftL1 loadWord;
-      loadDouble := liftL1 loadDouble;
-      storeByte   := liftL2 storeByte;
-      storeHalf   := liftL2 storeHalf;
-      storeWord   := liftL2 storeWord;
-      storeDouble := liftL2 storeDouble;
-      step := liftL0 step;
-      getCSRField_MTVecBase := liftL0 getCSRField_MTVecBase;
-      endCycle A := Return None;
-  |}.
-
-  Definition putProgram(prog: list (word 32))(ma: HarvardMachine): HarvardMachine :=
-    with_machine (putProgram prog ma.(machine)) ma.
-
-  Definition loadInst(addr: word wXLEN): OState HarvardMachine Instruction :=
-    im <- gets instructionMem;
-    Return (im addr).
-
   (* assumes generic translate and raiseException functions *)
-  Context {RVS: RiscvState (OState HarvardMachine) (word wXLEN)}.
+  Context {RVS: RiscvState (OState RiscvMachine) (word wXLEN)}.
   
-  Definition run1: OState HarvardMachine unit :=
+  Definition run1(imem: InstructionMem): OState RiscvMachine unit :=
     pc <- getPC;
-    inst <- loadInst pc;
-    execute inst;;
+    execute (imem pc);;
     step.
 
-  Definition run: nat -> OState HarvardMachine unit :=
-    fun n => power_func (fun m => run1 ;; m) n (Return tt).
+  Definition run(imem: InstructionMem): nat -> OState RiscvMachine unit :=
+    fun n => power_func (fun m => run1 imem ;; m) n (Return tt).
   
 End Riscv.
-
-Existing Instance IsHarvardMachine. (* needed because it was defined inside a Section *)
